Initial

btree.dfy
@@ -1,189 +1,14 @@
+include "Option.dfy"
+include "NativeInts.dfy"
+include "Vector.dfy"
 
 type Key = int
 type PageNumber = int
-datatype Option<T> = None | Some(value: T)
 datatype LeafCell<T> = LeafCell(key: Key, value: T)
 datatype InnerCell = InnerCell(key: Key, child: PageNumber)
 datatype Cell<T> = Cell(key: Key, value: T)
 
-newtype {:nativeType "uint"} u32 = x | 0 <= x < 0x1_0000_0000
-newtype {:nativeType "ulong"} u64 = x | 0 <= x < 0x1_0000_0000_0000_0000
 
-class Vector<T>
-{
-    var cells: array?<T>;
-    var used: u64;
-
-    constructor ()
-        ensures Valid()
-        ensures this.used == 0
-        ensures this.cells == null
-    {
-        this.used := 0;
-        this.cells := null;
-    }
-
-    function Valid() : bool
-        reads this
-    {
-        if this.cells == null then 
-            this.used == 0
-        else (
-            (0 < this.cells.Length < 0x1_0000_0000_0000_0000) &&
-            (0 <= used <= cells.Length as u64)
-        )
-    }
-
-    method try_pop() returns (value: Option<T>)
-        requires Valid()
-        modifies this, this.cells
-        ensures Valid()
-        ensures if old(this.used) > 0 then (
-            (this.used == (old(this.used) - 1)) &&
-            (value == Some(old(this.cells[this.used-1])))
-        ) else (
-            (this.used == old(this.used)) &&
-            (value == None)
-        )
-    {
-        if (this.cells != null && this.used > 0) {
-            this.used := this.used - 1;
-            return Some(this.cells[this.used]);
-        } else {
-            return None;
-        }
-    }
-
-    method push(value: T)
-        requires Valid()
-        requires this.used < 0xFFFF_FFFF_FFFF_FFFF
-        modifies this, this.cells
-        ensures Valid()
-        ensures this.cells != null
-        ensures old(this.used) + 1 == this.used
-        ensures old(this.cells == null) || old(this.cells[..this.used]) == this.cells[..(this.used-1)]
-        ensures this.cells[this.used - 1] == value
-        //ensures old(this.cells == null) || old(this.used == this.cells.Length as u64) || old(this.cells[this.used+1..]) == this.cells[this.used..]
-    {
-        if (cells == null || used == cells.Length as u64)
-        {
-            var len: u64 := 
-                if cells == null 
-                then 0 as u64
-                else this.cells.Length as u64;
-
-            var newLen: u64;
-            if (len == 0) {
-                newLen := 1;
-            } else if (len < 0x8000_0000_0000_0000 as u64) {
-                newLen := len * 2;
-            } else {
-                newLen := 0xFFFF_FFFF_FFFF_FFFF as u64;
-            }
-
-            var a := new T[newLen]((ii: int) reads this,cells => (
-                assume 0 <= ii < newLen as int;
-                var i: u64 := ii as u64;
-                assume cells == null || len as int == cells.Length;
-                if cells == null then
-                    value
-                else if 0 <= i < len then
-                    cells[i]
-                else
-                    value
-            ));
-
-            this.cells := a;
-        }
-
-        this.cells[used] := value;
-        used := used + 1 as u64;
-    }
-
-    function sequence() : (s: seq<T>)
-        requires Valid()
-        reads this, this.cells
-    {
-        if this.cells == null then [] else this.cells[..this.used]
-    }
-}
-
-method vector_test() 
-{
-    var v := new Vector<int>();
-
-    assert [] == v.sequence();
-
-    var i: Option<int>;
-    i := v.try_pop();
-    assert i == None;
-
-    v.push(1);
-    assert [1] == v.sequence();
-
-    // i := v.try_pop();
-    // assert Some(1) == i;
-}
-
-// class Span<T>
-// {
-//     var Array: array<T>;
-//     var Offset: int;
-//     var Count: int;
-
-//     function Valid() : bool 
-//         reads this
-//     {
-//         (0 <= Offset < Array.Length) &&
-//         (0 <= Count < Array.Length) &&
-//         (Offset + Count <= Array.Length)
-//     }
-
-//     function before() : (s: seq<T>)
-//         requires Valid()
-//         reads this, this.Array
-//     {
-//         Array[..Offset]
-//     }
-
-//     function after() : (s: seq<T>)
-//         requires Valid()
-//         reads this, this.Array
-//     {
-//         Array[Offset+Count..]
-//     }
-
-//     function method sequence() : (s: seq<T>)
-//         requires Valid()
-//         reads this, this.Array
-//     {
-//         Array[Offset..Offset+Count]
-//     }
-
-//     function method get(idx: int) : (v: T)
-//         requires Valid()
-//         requires 0 <= idx < Count
-//         reads this, this.Array
-//         ensures this.Array[Offset+idx] == v
-//     {
-//         Array[Offset+idx]
-//     }
-
-//     method put(idx: int, v: T)
-//         requires Valid()
-//         requires 0 <= idx < Count
-//         modifies this.Array
-//         ensures old(Array.Length) == Array.Length
-//         ensures old(before()) == before()
-//         ensures old(sequence()[..idx]) == sequence()[..idx]
-//         ensures v == sequence()[idx]
-//         ensures old(sequence()[idx+1..]) == sequence()[idx+1..]
-//         ensures old(after()) == after()
-//     {
-//         Array[Offset+idx] := v;
-//     }
-
-// }
 
 // method push_front<T>(s: Span<T>, v: T)
 //     requires s.Valid()
@@ -250,87 +75,77 @@ method vector_test()
 // }
 
 
-// class Node<T> {
-//     var cells: array<Option<Cell<T>>>;
-//     var used: int;
+class Node<T> {
+    var cells: Vector<Cell<T>>;
 
-//     constructor ()
-//         ensures invariants()
-//     {
-//         var len := 10;
-//         var c := new Option<Cell<T>>[len];
-//         forall (i | 0 <= i < len) {
-//             c[i] := None;
-//         }
-//         cells := c;
-//         used := 0;
-//     }
+    constructor ()
+        ensures Valid()
+    {
+        cells := new Vector<Cell<T>>();
+    }
 
-//     function invariants() : bool
-//         reads this, this.cells
-//     {
-//         (0 <= used <= cells.Length) &&
-//         (forall i :: 0 <= i < used ==> cells[i] != None) &&
-//         (forall i :: used <= i < cells.Length ==> cells[i] == None) &&
-//         (forall i :: 0 <= i < used ==> 
-//             (forall j :: 0 <= j < i ==> cells[j].value.key < cells[i].value.key)
-//         )
-//     }
+    predicate Valid()
+        reads this, this.cells
+    {
+        (cells.Length() == 0) ||
+        (forall i :: 0 <= i <= cells.MaxIndex() ==> 
+            (forall j :: 0 <= j < i ==> cells.get(j).key < cells.get(i).key)
+        )
+    }
 
 
-//     method insert(key: Key, value: T) returns (idx: int)
-//         requires invariants()
-//         requires used < cells.Length
-//         modifies this, cells
-//         ensures invariants()
-//         ensures idx < used
-//         ensures old(cells.Length) == cells.Length
-//         ensures idx >= 0 ==> 
-//             (old(used) + 1 == used) &&
-//             (old(cells[0..idx]) == cells[0..idx]) &&
-//             (forall i :: 0 <= i < idx ==> cells[i].value.key < key) && 
-//             (cells[idx] == Some(Cell(key,value))) &&
-//             (old(cells[idx..(cells.Length-1)]) == cells[(idx+1)..]) &&
-//             (forall i :: idx < i < used ==> key < cells[i].value.key)   
-//         ensures idx < 0 ==>
-//             (old(cells[..]) == cells[..]) &&
-//             (old(used) == used)
-//     {
-//         ghost var orig := cells[..];
+    method insert(key: Key, value: T) returns (idx: int)
+        requires Valid()
+        modifies this.cells
+        ensures Valid()
+        ensures idx < used
+        ensures old(cells.Length) == cells.Length
+        ensures idx >= 0 ==> 
+            (old(used) + 1 == used) &&
+            (old(cells[0..idx]) == cells[0..idx]) &&
+            (forall i :: 0 <= i < idx ==> cells[i].value.key < key) && 
+            (cells[idx] == Some(Cell(key,value))) &&
+            (old(cells[idx..(cells.Length-1)]) == cells[(idx+1)..]) &&
+            (forall i :: idx < i < used ==> key < cells[i].value.key)   
+        ensures idx < 0 ==>
+            (old(cells[..]) == cells[..]) &&
+            (old(used) == used)
+    {
+        ghost var orig := cells[..];
 
-//         idx := 0;
-//         while idx < used && cells[idx].value.key < key
-//             decreases used - idx
-//             invariant orig[..] == cells[..]
-//             invariant 0 <= idx < cells.Length
-//             invariant idx <= used
-//             invariant forall j :: 0 <= j < idx ==> cells[j] != None && cells[j].value.key < key
-//         {
-//             idx := idx + 1;
-//         }
+        idx := 0;
+        while idx < used && cells[idx].value.key < key
+            decreases used - idx
+            invariant orig[..] == cells[..]
+            invariant 0 <= idx < cells.Length
+            invariant idx <= used
+            invariant forall j :: 0 <= j < idx ==> cells[j] != None && cells[j].value.key < key
+        {
+            idx := idx + 1;
+        }
 
-//         assert forall j :: 0 <= j < idx ==> cells[j] != None && cells[j].value.key < key;
-//         if (idx == used) // add to end
-//         {
-//             assert cells[idx] == None;
-//             cells[idx] := Some(Cell(key, value));
-//             used := used + 1;
-//             return idx;
-//         }
+        assert forall j :: 0 <= j < idx ==> cells[j] != None && cells[j].value.key < key;
+        if (idx == used) // add to end
+        {
+            assert cells[idx] == None;
+            cells[idx] := Some(Cell(key, value));
+            used := used + 1;
+            return idx;
+        }
 
-//         assert idx < used;
-//         assert cells[idx] != None;
-//         if (cells[idx].value.key == key) // conflict
-//         {
-//             return -1;
-//         }
+        assert idx < used;
+        assert cells[idx] != None;
+        if (cells[idx].value.key == key) // conflict
+        {
+            return -1;
+        }
 
-//         assert invariants();
-//         used := used + 1;
-//         insert_at(cells, idx, Some(Cell(key,value)));
-//         return idx;
-//     }
-// }
+        assert invariants();
+        used := used + 1;
+        insert_at(cells, idx, Some(Cell(key,value)));
+        return idx;
+    }
+}
 
 // class LeafNode<T>
 // {
