List.dfy
@@ -1,0 +1,149 @@
+include "./Option.dfy"
+include "./NativeInts.dfy"
+
+class ListEntry<T>
+{
+    constructor Single(v: T)
+        ensures this.value == v;
+        ensures this.next == null;
+        ensures this.Contents == [v]
+        ensures this.Repr == {this}
+        ensures Valid()
+    {
+        this.value := v;
+        this.next := null;
+        this.Contents := [v];
+        this.Repr := {this};
+    }
+
+    constructor Prepend(v: T, n: ListEntry<T>)
+        requires n.Valid()
+        ensures this.value == v;
+        ensures this.next == n;
+        ensures this.Contents == [v] + n.Contents
+        ensures this.Repr == {this} + n.Repr
+        ensures Valid()
+    {
+        this.value := v;
+        this.next := n;
+        this.Contents := [v] + n.Contents;
+        this.Repr := {this} + n.Repr;
+    }
+
+    var value: T;
+    var next: ListEntry?<T>;
+
+    ghost var Contents: seq<T>
+    ghost var Repr: set<object>
+
+    predicate Valid()
+        reads this, Repr
+        decreases Repr
+    {
+        this in Repr &&
+        1 <= |Contents| && Contents[0] == value &&
+        (next == null ==> |Contents| == 1) &&
+        (next != null ==> 
+            next in Repr &&
+            Repr > next.Repr &&
+            this !in next.Repr && // not a loop
+            next.Valid() &&
+            next.Contents == Contents[1..]
+        )
+    }
+
+    function Tail() : ListEntry<T>
+        requires Valid()
+        reads this, this.Repr
+        decreases this.Repr //if this.next == null then {} else this.Repr
+    {
+        if this.next == null
+            then this
+            else this.next.Tail()
+    }
+}
+
+class List<T>
+{
+    var first: ListEntry?<T>;
+    var last: ListEntry?<T>;
+
+    predicate Valid() 
+        reads this,
+            first, if first != null then first.Repr else {},
+            last, if last != null then last.Repr else {}
+    {
+        ((first == null) ==> 
+            last == null
+        ) &&
+        ((first != null) ==> 
+            first.Valid() &&
+            this !in first.Repr &&
+            last != null && 
+            last.Valid() &&
+            this !in last.Repr &&
+            last.next == null &&
+            this.first.Tail() == last
+        )
+
+    }
+
+    constructor()
+        ensures Valid()
+    {
+        this.first := null;
+        this.last := null;
+    }
+
+    constructor from(v: T)
+        ensures Valid()
+    {
+        this.first := new ListEntry<T>.Single(v);
+        this.last := this.first;
+    }
+
+    function Sequence() : seq<T>
+        reads this, this.first
+    {
+        if this.first == null then [] else this.first.Contents
+    }
+
+    method prepend(v: T)
+        requires Valid()
+        modifies this
+        ensures Valid()
+        ensures [v] + old(this.Sequence()) == this.Sequence()
+    {
+        var n : ListEntry<T>;
+        if (this.first == null) {
+            n := new ListEntry<T>.Single(v);
+            this.first := n;
+            this.last := n;
+        } else {
+            n := new ListEntry<T>.Prepend(v, this.first);
+            this.first := n;
+        }
+    }
+
+    // method append(v: T)
+    //     requires Valid()
+    //     modifies this, this.last
+    //     ensures Valid()
+    // {
+    //     var n := new ListEntry<T>.Single(v);
+    //     if (this.first == null) {
+    //         this.first := n;
+    //         this.last := n;
+    //     } else {
+    //         this.last.next := n;
+    //     }
+    // }
+}
+
+method ListTest()
+{
+    var l := new List<int>();
+    l.prepend(3);
+    l.prepend(2);
+    l.prepend(1);
+}
