NativeInts.dfy
@@ -1,0 +1,18 @@
+newtype {:nativeType "int"} i32 = x | -0x8000_0000 <= x < 0x8000_0000
+newtype {:nativeType "uint"} u32 = x | 0 <= x < 0x1_0000_0000
+newtype {:nativeType "ulong"} u64 = x | 0 <= x < 0x1_0000_0000_0000_0000
+
+newtype {:nativeType "int"} ArrayIndex = x | 0 <= x < 0x7FF0_0000
+newtype {:nativeType "int"} ArrayLength = x | 0 <= x < 0x7FF0_0001
+
+
+class NativeIntConstants {
+    static const MaxArrayLengthInt := 0x7FF0_0000;
+    static const MaxArrayIndexInt := 0x7FEF_FFFF;
+    static const MaxArrayIndex: ArrayIndex := MaxArrayIndexInt as ArrayIndex;
+    static const MaxArrayLength: ArrayLength := MaxArrayLengthInt as ArrayLength;
+
+    ghost method checks() {
+        assert MaxArrayIndexInt + 1 == MaxArrayLengthInt;
+    }
+}
