Option.dfy
@@ -1,0 +1,1 @@
+datatype Option<T> = None | Some(value: T)
