Span.dfy
@@ -1,0 +1,128 @@
+include "NativeInts.dfy"
+
+class Span<T>
+{
+    var Array: array<T>;
+    var Offset: ArrayIndex;
+    var Count: ArrayLength;
+
+    constructor(a: array<T>, offset: ArrayIndex, count: ArrayLength)
+        requires ValidRange(a, offset, count)
+        ensures Array == a && Offset == offset && Count == count
+        ensures Array.Length == a.Length
+        ensures forall i :: 0 <= i < Array.Length ==> Array[i] == a[i]
+        ensures Valid()
+    {
+        Array := a;
+        Offset := offset;
+        Count := count;
+    }
+
+    static predicate ValidRange(a: array<T>, offset: ArrayIndex, count: ArrayLength)
+    {
+        (0 <= offset as int < a.Length) &&
+        (0 <= offset as int < a.Length) &&
+        (offset as int + count as int <= a.Length) &&
+        (offset <= NativeIntConstants.MaxArrayIndex) &&
+        (count <= NativeIntConstants.MaxArrayLength) &&
+        (offset as int + count as int <= NativeIntConstants.MaxArrayLengthInt)
+    }
+
+    predicate Valid()
+        reads this
+    {
+        ValidRange(Array, Offset, Count)
+    }
+
+    function before() : (s: seq<T>)
+        requires Valid()
+        reads this, this.Array
+    {
+        Array[..Offset]
+    }
+
+    static function index_offset(i: ArrayIndex, o: ArrayLength) : (ii: ArrayIndex)
+        requires o as int <= NativeIntConstants.MaxArrayIndexInt
+        requires (i as int) + (o as int) <= NativeIntConstants.MaxArrayIndexInt
+        ensures (ii as int) == (i as int) + (o as int)
+    {
+        i+(o as ArrayIndex)
+    }
+
+    function after() : (s: seq<T>)
+        requires Valid()
+        reads this, this.Array
+    {
+        if (NativeIntConstants.MaxArrayLength - Count == Offset as ArrayLength)
+            then []
+            else Array[index_offset(Offset, Count)..]
+    }
+
+    function sequence() : (s: seq<T>)
+        requires Valid()
+        reads this, this.Array
+        ensures |s| == Count as int
+        ensures forall i :: 0 <= i < Count as int ==> s[i] == Array[i + Offset as int]
+    {
+        if (NativeIntConstants.MaxArrayLength - Count == Offset as ArrayLength)
+            then Array[Offset..NativeIntConstants.MaxArrayLengthInt]
+            else Array[Offset..index_offset(Offset, Count)]
+    }
+
+    function method get(idx: ArrayIndex) : (v: T)
+        requires Valid()
+        requires 0 <= idx as int < Count as int
+        reads this, this.Array
+        ensures this.Array[Offset+idx] == v
+    {
+        Array[Offset+idx]
+    }
+
+    method put(idx: ArrayIndex, v: T)
+        requires Valid()
+        requires 0 <= idx as int < Count as int
+        modifies this.Array
+        ensures old(Array.Length) == Array.Length
+        ensures old(before()) == before()
+        ensures old(sequence()[..idx]) == sequence()[..idx]
+        ensures v == sequence()[idx]
+        ensures idx == NativeIntConstants.MaxArrayIndex || old(sequence()[idx+1..]) == sequence()[idx+1..]
+        ensures old(after()) == after()
+    {
+        Array[Offset+idx] := v;
+    }
+
+    method subspan(i: ArrayIndex, c: ArrayLength) returns (s: Span<T>)
+        requires Valid()
+        requires 0 <= i as int < Count as int
+        requires 0 <= c < Count
+        requires ValidRange(Array, Offset + i, c)
+        requires 0 <= i as int + c as int <= Count as int
+        ensures fresh(s)
+        ensures s.Array == this.Array
+        ensures s.Offset == this.Offset + i
+        ensures s.Count == c
+        ensures s.Valid()
+        ensures s.sequence() == this.sequence()[i..i as int + c as int]
+    {
+        s := new Span<T>(Array, Offset + i, c);
+    }
+}
+
+method SpanTest()
+{
+    var a := new i32[4];
+    a[0 as ArrayIndex] := 0 as i32;
+    a[1 as ArrayIndex] := 1 as i32;
+    a[2 as ArrayIndex] := 2 as i32;
+    a[3 as ArrayIndex] := 3 as i32;
+
+    var s1 := new Span<i32>(a, 0, 1);
+    assert s1.sequence() == [0];
+
+    var s2 := new Span<i32>(a, 2, 2);
+    assert s2.sequence() == [2,3];
+
+    var s3 := s2.subspan(1,1);
+    assert s3.sequence() == [3];
+}
