Vector.dfy
@@ -1,0 +1,247 @@
+include "Option.dfy"
+include "NativeInts.dfy"
+
+class Vector<T>
+{
+    var cells: array?<T>;
+    var used: ArrayLength;
+
+    constructor ()
+        ensures Valid()
+        ensures this.used == 0
+        ensures this.cells == null
+    {
+        this.used := 0;
+        this.cells := null;
+    }
+
+    predicate Valid()
+        reads this
+    {
+        if this.cells == null then
+            this.used == 0
+        else (
+            (0 < this.cells.Length) &&
+            (this.cells.Length <= NativeIntConstants.MaxArrayLengthInt) &&
+            (0 <= used <= cells.Length as ArrayLength)
+        )
+    }
+
+    function method MaxIndex() : (i: ArrayIndex)
+        requires this.used > 0
+        requires Valid()
+        reads this
+        ensures i as int < this.cells.Length
+    {
+        (this.used - 1) as ArrayIndex
+    }
+
+    function Length() : ArrayLength
+        reads this
+    {
+        this.used
+    }
+
+    method try_pop() returns (value: Option<T>)
+        requires Valid()
+        modifies this, this.cells
+        ensures Valid()
+        ensures old(this.cells) == this.cells
+        ensures if old(this.used) > 0 then (
+            (this.used == (old(this.used) - 1)) &&
+            (value == Some(old(this.cells[this.used-1]))) &&
+            (old(this.sequence()[..this.used-1]) == this.sequence()[..this.used])
+        ) else (
+            (this.used == old(this.used)) &&
+            (value == None) &&
+            (old(this.sequence()) == this.sequence())
+        )
+    {
+        if (this.cells != null && this.used > 0) {
+            this.used := this.used - 1;
+            return Some(this.cells[this.used]);
+        } else {
+            return None;
+        }
+    }
+
+    method alloc(value: T)
+        requires Valid()
+        requires this.cells == null
+        modifies this
+        ensures Valid()
+        ensures old(used) == used
+        ensures this.cells != null && this.cells[..] == [value]
+        ensures fresh(this.cells)
+    {
+        this.cells := new T[1](_ => value);
+    }
+
+    method allocOrGrow(value: T)
+        requires Valid()
+        requires this.cells == null || (
+            this.used as int == this.cells.Length &&
+            this.cells.Length < NativeIntConstants.MaxArrayLengthInt
+            )
+        modifies this
+        ensures Valid()
+        ensures old(this.used) == this.used
+        ensures this.cells != null
+        ensures fresh(this.cells)
+        ensures old(this.sequence()) == this.sequence()[..this.used]
+        ensures this.cells.Length > this.used as int
+    {
+        if (this.cells == null) {
+            this.alloc(value);
+        } else {
+            this.grow(value);
+        }
+    }
+
+    method grow(filler: T)
+        requires Valid()
+        requires this.cells != null
+        requires this.used as int == this.cells.Length
+        requires this.cells.Length < NativeIntConstants.MaxArrayLengthInt
+        modifies this
+        ensures Valid()
+        ensures old(used) == used
+        ensures this.cells != null
+        ensures fresh(this.cells)
+        ensures this.cells.Length > old(this.cells.Length)
+        ensures old(this.cells[..]) == this.cells[..old(this.cells.Length)]
+    {
+        var len := this.cells.Length as ArrayLength;
+
+        var newLen: ArrayLength;
+        if (len < NativeIntConstants.MaxArrayLength / (2 as ArrayLength)) {
+            newLen := len * 2;
+        } else {
+            newLen := NativeIntConstants.MaxArrayLength;
+        }
+
+        var a := new T[newLen]((ii: int) reads this,cells => (
+            assume 0 <= ii <= NativeIntConstants.MaxArrayIndex as int;
+            var i: ArrayIndex := ii as ArrayIndex;
+            assume cells == null || len as int == cells.Length;
+            if cells == null then
+                filler
+            else if (i as ArrayLength) < len then
+                cells[i]
+            else
+                filler
+        ));
+
+        this.cells := a;
+    }
+
+    method insert_at(idx: ArrayIndex, value: T)
+        requires Valid()
+        requires this.used < NativeIntConstants.MaxArrayLength
+        requires 0 <= idx as ArrayLength < this.Length()
+        modifies this, this.cells
+        ensures Valid()
+        ensures this.cells != null
+        ensures (old(this.cells) != this.cells) ==> fresh(this.cells)
+        ensures old(this.used) + 1 == this.used
+        ensures old(this.cells == null) ==> (
+            this.cells.Length == 1 &&
+            this.cells[0] == value
+        )
+        ensures old(this.cells != null) ==> (
+            (old(this.cells.Length) <= this.cells.Length) &&
+            (old(this.cells[..idx]) == this.cells[..idx]) &&
+            (old(this.cells[idx..this.used]) == this.cells[idx+1..this.used])
+        )
+        ensures this.cells[idx] == value
+    {
+        ghost var orig := this.cells[..];
+
+        if (cells == null || used == cells.Length as ArrayLength)
+        {
+            this.allocOrGrow(value);
+            assert orig[..idx] == this.cells[..idx];
+        }
+
+        assert orig[..idx] == this.cells[..idx];
+
+        this.used := this.used + 1;
+        var dst := this.MaxIndex();
+        assert idx <= dst;
+        while dst > idx
+            decreases dst as int - idx as int
+            modifies this.cells
+            invariant Valid()
+            invariant this.cells != null
+            invariant orig[..idx] == this.cells[..idx]
+            invariant orig[used..] == this.cells[used..]
+            invariant idx as int <= dst as int < this.used as int <= this.cells.Length
+        {
+            this.cells[dst] := this.cells[dst - 1];
+            dst := dst - 1;
+        }
+
+        assert this.cells != null;
+
+        this.cells[idx] := value;
+    }
+
+    method push(value: T)
+        requires Valid()
+        requires this.used < NativeIntConstants.MaxArrayLength
+        modifies this, this.cells
+        ensures Valid()
+        ensures this.cells != null
+        ensures (old(this.cells) != this.cells) ==> fresh(this.cells)
+        ensures old(this.used) + 1 == this.used
+        ensures old(this.cells == null) || old(this.cells[..this.used]) == this.cells[..(this.used-1)]
+        ensures this.cells[this.used - 1] == value
+    {
+        if (cells == null || used == cells.Length as ArrayLength)
+        {
+            this.allocOrGrow(value);
+        }
+
+        this.cells[used] := value;
+        used := used + 1 as ArrayLength;
+    }
+
+    function sequence() : (s: seq<T>)
+        requires Valid()
+        reads this, this.cells
+        ensures |s| <= NativeIntConstants.MaxArrayLengthInt
+        ensures |s| as ArrayLength == this.used
+    {
+        if this.cells == null then [] else this.cells[..this.used]
+    }
+
+    function method get(i: ArrayIndex) : T
+        requires Valid()
+        requires i as ArrayLength < this.used
+        reads this, this.cells
+    {
+        this.cells[i]
+    }
+}
+
+// method vector_test()
+// {
+//     var v := new Vector<int>();
+
+//     assert [] == v.sequence();
+
+//     v.push(0);
+//     assert [0] == v.sequence();
+
+//     v.push(1);
+//     assert [0, 1] == v.sequence();
+
+//     var i := v.try_pop();
+//     assert Some(1) == i;
+
+//     i := v.try_pop();
+//     assert Some(0) == i;
+
+//     i := v.try_pop();
+//     assert None == i;
+// }
