all.dfy
@@ -1,0 +1,5 @@
+include "List.dfy"
+include "NativeInts.dfy"
+include "Option.dfy"
+include "Span.dfy"
+include "Vector.dfy"
